added a standard STS for reasoning about shared memory

theories/logrel.v
@@ -9,19 +9,21 @@ Import uPred.
 (** CMRA for heap and its predicates. Contains: *)
 (* CMRA for relatedness between locations and saved prop names *)
 (* CMRA for saved predicates *)
-Definition relUR : ucmraT := gmapUR Addr (agreeR (prodO gnameO (leibnizO Perm))).
+Definition relUR : ucmraT := gmapUR Addr (agreeR (leibnizO (gname * Perm))).
+Definition relT := gmap Addr (leibnizO (gname * Perm)). 
 
 Class heapG Σ := HeapG {
   heapG_invG : invG Σ;
-  heapG_saved_pred :> savedPredG Σ ((STS_states * STS_rels) * Word);
+  heapG_saved_pred :> savedPredG Σ (((STS_states * STS_rels) * (STS_states * STS_rels)) * Word);
   heapG_rel :> inG Σ (authR relUR);
   γrel : gname
 }.
 
 Section heap.
-  Context `{heapG Σ, memG Σ, regG Σ,
+  Context `{heapG Σ, memG Σ, regG Σ, STSG Σ,
             MonRef: MonRefG (leibnizO _) CapR_rtc Σ}.
-  Notation WORLD := (leibnizO (STS_states * STS_rels)).
+  Notation STS := (leibnizO (STS_states * STS_rels)).
+  Notation WORLD := (prodO STS STS). 
   Implicit Types W : WORLD.
   
   Definition REL_def l p γ : iProp Σ := own γrel (◯ {[ l := to_agree (γ,p) ]}).
@@ -29,7 +31,7 @@ Section heap.
   Definition REL := proj1_sig REL_aux.
   Definition REL_eq : @REL = @REL_def := proj2_sig REL_aux.
   
-  Definition RELS_def (M : relUR) : iProp Σ := own γrel (● M).
+  Definition RELS_def (M : relT) : iProp Σ := own γrel (● (to_agree <$> M : relUR)).
   Definition RELS_aux : { x | x = @RELS_def }. by eexists. Qed.
   Definition RELS := proj1_sig RELS_aux.
   Definition RELS_eq : @RELS = @RELS_def := proj2_sig RELS_aux.
@@ -45,25 +47,123 @@ Section heap.
     Persistent (rel l p φ).
   Proof. rewrite rel_eq /rel_def REL_eq /REL_def. apply _. Qed.
   
-  Definition future_mono (φ : ((STS_states * STS_rels) * Word) -> iProp Σ) : iProp Σ :=
-    (□ ∀ W W' v, ⌜related_sts_pub W.1 W'.1 W.2 W'.2⌝ → φ (W,v) -∗ φ (W',v))%I. 
-  
-  Definition region_def W : iProp Σ := 
-    (∃ (M : relUR), RELS M
-                         ∗ [∗ map] a↦γp ∈ M, ∃ γpred (v : Word) (p : Perm) φ,
-                                               ⌜γp = to_agree (γpred,p)⌝
+  Definition future_pub_mono (φ : (WORLD * Word) -> iProp Σ) v : iProp Σ :=
+    (□ ∀ W W', ⌜related_sts_pub_world W W'⌝ → φ (W,v) -∗ φ (W',v))%I.
+
+  Definition future_priv_mono (φ : (WORLD * Word) -> iProp Σ) v : iProp Σ :=
+    (□ ∀ W W', ⌜related_sts_priv_world W W'⌝ → φ (W,v) -∗ φ (W',v))%I.
+
+  Definition pwl p : bool :=
+    match p with
+    | RWLX | RWL => true
+    | _ => false
+    end.
+
+  (* We will first define the standard STS for the shared part of the heap *)
+  Inductive region_type :=
+  | Temporary
+  | Permanent
+  | Revoked.
+
+  Global Instance region_type_EqDecision : EqDecision region_type.
+  Proof.
+    intros ρ1 ρ2.
+    destruct ρ1,ρ2;
+      [by left|by right|by right|by right|
+         by left|by right|by right|by right|by left]. 
+  Qed.
+  Global Instance region_type_finite : finite.Finite region_type.
+  Proof.
+    refine {| finite.enum := [Temporary; Permanent; Revoked] ;
+              finite.NoDup_enum := _ ;
+              finite.elem_of_enum := _ |}.
+    - repeat (apply NoDup_cons; split; [repeat (apply not_elem_of_cons;split;auto); apply not_elem_of_nil|]).
+        by apply NoDup_nil.
+    - intros ρ.
+      destruct ρ;apply elem_of_cons;[by left|right|right];
+        apply elem_of_cons;[by left|right];
+          apply elem_of_cons; by left. 
+  Qed.           
+  Global Instance region_type_countable : Countable region_type.
+  Proof. apply finite.finite_countable. Qed. 
+
+  Definition std_rel_pub := λ a b, (a = Revoked ∧ b = Temporary).
+  Definition std_rel_priv := λ a b, a = Temporary ∨ b = Permanent.
+  Global Instance sts_std : STS_STD region_type := {| Rpub := std_rel_pub; Rpriv := std_rel_priv |}. 
+
+  (* Some practical shorthands for projections *)
+  Definition std W := W.1.
+  Definition loc W := W.2.
+  Definition std_sta W := W.1.1.
+  Definition std_rel W := W.1.2.
+
+  Definition dom_equal (Wstd_sta : STS_states) (M : relT) :=
+    ∀ (i : positive), is_Some (Wstd_sta !! i) ↔ (∃ (a : Addr), countable.encode a = i ∧ is_Some (M !! a)).
+
+  Lemma dom_equal_empty : dom_equal ∅ ∅.
+  Proof.
+    rewrite /dom_equal =>a.
+    split; intros [x Hx]; [inversion Hx|destruct Hx as [_ Hx];by inversion Hx]. 
+  Qed.
+
+  Lemma dom_equal_insert Wstd_sta M (a : Addr) x y :
+    dom_equal Wstd_sta M → dom_equal (<[countable.encode a := x]> Wstd_sta) (<[a := y]> M).
+  Proof.
+    intros Heq.
+    rewrite /dom_equal =>i.
+    split; intros [z Hz]. 
+    - destruct (decide ((countable.encode a) = i)); subst.
+      { exists a. split;[auto|]. rewrite lookup_insert. eauto. }
+      { rewrite lookup_insert_ne in Hz; auto.
+        destruct Heq with i as [Heq_i _].
+        destruct Heq_i as [a' [Ha' HMa'] ]; eauto.
+        exists a'; split;[auto|]. rewrite lookup_insert_ne; auto.
+        intros Ha. subst. done. 
+      }
+    - destruct Hz as [Hi Hz]. 
+      destruct (decide ((countable.encode a) = i)); subst.
+      { rewrite e. rewrite lookup_insert. eauto. }
+      { rewrite lookup_insert_ne;auto.
+        destruct Heq with (countable.encode z) as [_ Heq_i].
+        apply Heq_i.
+        exists z. split; auto.
+        rewrite lookup_insert_ne in Hz; auto.
+        intros Ha; congruence. 
+      }
+  Qed.
+
+  Definition region_map_def M W :=
+    ([∗ map] a↦γp ∈ M, ∃ ρ, sts_state_std (countable.encode a) ρ ∗
+                            match ρ with
+                            | Temporary => ∃ γpred (v : Word) (p : Perm) φ,
+                                               ⌜γp = (γpred,p)⌝
                                              ∗ ⌜p ≠ O⌝
-                                             ∗ (a ↦ₐ[p] v)
-                                             ∗ future_mono φ
+                                             ∗ a ↦ₐ[p] v
+                                             ∗ (if pwl p
+                                               then future_pub_mono φ v
+                                               else future_priv_mono φ v)
                                              ∗ saved_pred_own γpred φ
-                                             ∗ ▷ φ (W,v))%I.
+                                             ∗ ▷ φ (W,v)
+                            | Permanent => ∃ γpred (v : Word) (p : Perm) φ,
+                                               ⌜γp = (γpred,p)⌝
+                                             ∗ ⌜p ≠ O⌝
+                                             ∗ a ↦ₐ[p] v
+                                             ∗ future_priv_mono φ v
+                                             ∗ saved_pred_own γpred φ
+                                             ∗ ▷ φ (W,v)
+                            | Revoked => emp
+                            end)%I. 
+        
+  Definition region_def W : iProp Σ := 
+    (∃ (M : relT), RELS M ∗ ⌜dom_equal (std_sta W) M⌝
+                         ∗ region_map_def M W)%I. 
   Definition region_aux : { x | x = @region_def }. by eexists. Qed.
   Definition region := proj1_sig region_aux.
   Definition region_eq : @region = @region_def := proj2_sig region_aux.
 
-  Lemma reg_in γ R n r:
-    (own γ (● R) ∗ own γ (◯ {[n := to_agree r]}) -∗
-        ⌜R = <[n := to_agree r]>(delete n R)⌝)%I.
+  Lemma reg_in γ (R : relT) (n : Addr) (r : leibnizO (gname * Perm)) :
+    (own γ (● (to_agree <$> R : relUR)) ∗ own γ (◯ {[n := to_agree r]}) -∗
+        ⌜R = <[n := r]>(delete n R)⌝)%I.
   Proof.
     iIntros "[H1 H2]".
     iDestruct (own_valid_2 with "H1 H2") as %Hv.
@@ -78,9 +178,12 @@ Section heap.
     revert Hi Heq; rewrite -Hy => Hi Heq.
     apply to_agree_included in Hi; subst.
     revert Heq; rewrite -Hi => Heq.
-    rewrite insert_delete insert_id; auto. eapply leibniz_equiv. apply Heq.
-    Unshelve. 
-  Admitted.
+    rewrite insert_delete insert_id /leibniz_equiv_iff => //; auto.
+    revert Heq. rewrite lookup_fmap fmap_Some_equiv =>Hx.
+    destruct Hx as [x [-> Hrx] ].
+    apply to_agree_inj, leibniz_equiv_iff in Hrx as ->. 
+    done. 
+  Qed. 
 
   Lemma rels_agree a γ1 γ2 p1 p2 :
     REL a p1 γ1 ∗ REL a p2 γ2 -∗ ⌜γ1 = γ2⌝ ∧ ⌜p1 = p2⌝.
@@ -91,7 +194,7 @@ Section heap.
     iPureIntro.
     rewrite -auth_frag_op op_singleton in Hval.
     apply singleton_valid in Hval.
-    apply agree_op_invL' in Hval.
+    apply (agree_op_invL' (A:=leibnizO _)) in Hval.
     by inversion Hval. 
   Qed. 
 
@@ -105,79 +208,431 @@ Section heap.
     iDestruct (rels_agree with "[$Hrel1 $Hrel2]") as %[-> ->].
     iSplitR;[auto|]. iIntros (x). iApply (saved_pred_agree with "Hpred1 Hpred2").
   Qed. 
-    
-  Lemma extend_region E W l p v φ `{∀ W v, Persistent (φ (W,v))}:
-    (⌜p ≠ O⌝ → future_mono φ →
-    region W -∗ l ↦ₐ[p] v -∗ φ (W,v) ={E}=∗ region W ∗ rel l p φ)%I.
+  
+  Definition temporary (W : WORLD) (l : Addr) :=
+    match W.1.1 !! (countable.encode l) with
+    | Some ρ => ρ = countable.encode Temporary
+    | _ => False
+    end.
+  Definition permanent (W : WORLD) (l : Addr) :=
+    match W.1.1 !! (countable.encode l) with
+    | Some ρ => ρ = countable.encode Permanent
+    | _ => False
+    end.
+  Definition revoked (W : WORLD) (l : Addr) :=
+    match W.1.1 !! (countable.encode l) with
+    | Some ρ => ρ = countable.encode Revoked
+    | _ => False
+    end.
+  
+  Definition std_update (W : WORLD) (l : Addr) (a : region_type) (r1 r2 : region_type → region_type -> Prop) : WORLD :=
+    ((<[countable.encode l := countable.encode a]>W.1.1,
+      <[countable.encode l := (convert_rel r1,convert_rel r2)]>W.1.2), W.2). 
+  Definition loc_update (W : WORLD) (l : Addr) (a : region_type) (r1 r2 : region_type → region_type -> Prop) : WORLD :=
+    (W.1,(<[countable.encode l := countable.encode a]>W.2.1,
+          <[countable.encode l := (convert_rel r1,convert_rel r2)]>W.2.2)).
+
+  Notation "<s[ a := ρ , r ]s> W" := (std_update W a ρ r.1 r.2) (at level 10, format "<s[ a := ρ , r ]s> W").
+  Notation "<l[ a := ρ , r ]l> W" := (loc_update W a ρ r.1 r.2) (at level 10, format "<l[ a := ρ , r ]l> W").
+
+  Definition open_region_def (a : Addr) (W : WORLD) : iProp Σ :=
+    (∃ (M : relT), RELS M ∗ ⌜dom_equal (std_sta W) M⌝ ∗ region_map_def (delete a M) W)%I. 
+  Definition open_region_aux : { x | x = @open_region_def }. by eexists. Qed.
+  Definition open_region := proj1_sig open_region_aux.
+  Definition open_region_eq : @open_region = @open_region_def := proj2_sig open_region_aux.
+
+  Lemma related_sts_pub_priv_world W W' :
+    related_sts_pub_world W W' -> related_sts_priv_world W W'.
   Proof.
-    iIntros (Hpne) "#Hmono Hreg Hl #Hφ".
+    intros [Hstd Hloc].
+    split; apply related_sts_pub_priv; auto.
+  Qed.
+
+  Lemma region_map_monotone W W' M :
+    (⌜related_sts_pub_world W W'⌝ →
+     region_map_def M W -∗ region_map_def M W')%I.
+  Proof.
+    iIntros (Hrelated) "Hr".
+    iApply big_sepM_mono; iFrame. 
+    iIntros (a γ Hsome) "Hm".
+    iDestruct "Hm" as (ρ) "[Hstate Hm]".
+    iExists ρ. iFrame. 
+    destruct ρ.
+    - iDestruct "Hm" as (γpred v p φ Heq HO) "(Hl & Hmono & #Hsavedφ & Hφ)".
+      iExists _,_,_,_. do 2 (iSplitR;[eauto|]).
+      destruct (pwl p);
+      (iDestruct "Hmono" as "#Hmono"; iFrame "∗ #";
+        iApply "Hmono"; iFrame; auto); 
+      try (iPureIntro; by apply related_sts_pub_priv_world).      
+    - iDestruct "Hm" as (γpred v p φ Heq HO) "(Hl & #Hmono & #Hsavedφ & Hφ)".
+      iExists _,_,_,_. do 2 (iSplitR;[eauto|]).
+      iFrame "∗ #".
+      iApply "Hmono"; iFrame; auto. 
+      iPureIntro. 
+      by apply related_sts_pub_priv_world. 
+    - done.
+  Qed. 
+    
+  Lemma region_monotone W W' :
+    (⌜dom (gset positive) (std_sta W) = dom (gset positive) (std_sta W')⌝ →
+     ⌜related_sts_pub_world W W'⌝ → region W -∗ region W')%I.
+  Proof.
+    iIntros (Hdomeq Hrelated) "HW". rewrite region_eq.
+    iDestruct "HW" as (M) "(HM & % & Hmap)". 
+    iExists (M). iFrame.
+    iApply (wand_frame_r _ emp%I).
+    { iIntros (_).
+      iPureIntro.
+      intros a. split; intros [x Hx].
+      - destruct H3 with a as [Hstd _].
+        apply Hstd. apply elem_of_gmap_dom.
+        rewrite Hdomeq. apply elem_of_gmap_dom. eauto.
+      - destruct H3 with a as [_ Hstd].
+        apply elem_of_gmap_dom. rewrite -Hdomeq.
+        apply elem_of_gmap_dom. eauto.
+    } iSplitR;[auto|].
+    iApply region_map_monotone; eauto. 
+  Qed.    
+    
+  Lemma related_sts_pub_world_fresh W a ρ :
+    (countable.encode a) ∉ dom (gset positive) (std_sta W) →
+    (countable.encode a) ∉ dom (gset positive) (std_rel W) →
+    related_sts_pub_world W (<s[a:=ρ,(Rpub,Rpriv)]s> W).
+  Proof.
+    rewrite /std_sta /std_rel. intros Hdom_sta Hdom_rel.
+    rewrite /related_sts_pub_world /=.
+    split;[|apply related_sts_pub_refl].
+    rewrite /related_sts_pub. split;[|split;[auto|] ]. 
+    - apply dom_insert_subseteq.
+    - apply dom_insert_subseteq. 
+    - apply not_elem_of_dom in Hdom_sta.
+      apply not_elem_of_dom in Hdom_rel.
+      intros i r1 r2 r1' r2' Hr Hr'. 
+      destruct (decide (countable.encode a = i)).
+      + subst. rewrite Hr in Hdom_rel. done. 
+      + rewrite lookup_insert_ne in Hr'; auto.
+        rewrite Hr in Hr'. inversion Hr'. repeat (split;auto).
+        intros x y Hx Hy. 
+        rewrite lookup_insert_ne in Hy;auto.
+        rewrite Hx in Hy. 
+        inversion Hy; inversion Hr'; subst.
+        left.
+  Qed.
+
+   Lemma related_sts_pub_world_fresh_state W a ρ :
+    (countable.encode a) ∉ dom (gset positive) (std_sta W) →
+    std_rel W !! (countable.encode a) = Some (convert_rel (Rpub : relation region_type),convert_rel (Rpriv : relation region_type)) →
+    related_sts_pub_world W (<s[a:=ρ,(Rpub,Rpriv)]s> W).
+  Proof.
+    rewrite /std_sta /std_rel. intros Hdom_sta Hdom_rel.
+    rewrite /related_sts_pub_world /=.
+    split;[|apply related_sts_pub_refl].
+    rewrite /related_sts_pub. split;[|split;[auto|] ]. 
+    - apply dom_insert_subseteq.
+    - apply dom_insert_subseteq. 
+    - apply not_elem_of_dom in Hdom_sta.
+      intros i r1 r2 r1' r2' Hr Hr'. 
+      destruct (decide (countable.encode a = i)).
+      + subst. rewrite Hr in Hdom_rel. rewrite lookup_insert in Hr'. simplify_eq.
+        repeat (split;auto). intros x y Hcontr. rewrite Hcontr in Hdom_sta. done. 
+      + rewrite lookup_insert_ne in Hr'; auto.
+        rewrite Hr in Hr'. inversion Hr'. repeat (split;auto).
+        intros x y Hx Hy. 
+        rewrite lookup_insert_ne in Hy;auto.
+        rewrite Hx in Hy. 
+        inversion Hy; inversion Hr'; subst.
+        left.
+  Qed. 
+  
+  Lemma extend_region_temp_pwl E W l p v φ `{∀ W v, Persistent (φ (W,v))}:
+     p ≠ O →
+     (countable.encode l) ∉ dom (gset positive) (std_sta W) →
+     (countable.encode l) ∉ dom (gset positive) (std_rel W) →
+     (pwl p) = true →
+     (future_pub_mono φ v →
+     sts_full_world sts_std W -∗ region W -∗ l ↦ₐ[p] v -∗ φ (W,v) ={E}=∗ region (<s[l := Temporary, (Rpub,Rpriv) ]s>W)
+                                                              ∗ rel l p φ
+                                                              ∗ sts_full_world sts_std (<s[l := Temporary, (Rpub,Rpriv)]s>W))%I.
+  Proof.
+    iIntros (Hpne Hnone1 Hnone2 Hpwl) "#Hmono Hfull Hreg Hl #Hφ".
     rewrite region_eq rel_eq /region_def /rel_def.
-    iDestruct "Hreg" as (M) "(Hγrel & Hpreds)".
+    iDestruct "Hreg" as (M) "(Hγrel & % & Hpreds)".
     rewrite RELS_eq /RELS_def. 
     (* destruct on M !! l *)
     destruct (M !! l) eqn:HRl.
-    { (* Cannot have two capability ghost resources: contradiction *)
+    { (* The location is not in the map *)
       iDestruct (big_sepM_delete _ _ _ _ HRl with "Hpreds") as "[Hl' _]".
-      iDestruct "Hl'" as (γpred' v' p' φ') "(_ & % & Hl' & _)".
-      by iDestruct (cap_duplicate_false with "[$Hl $Hl']") as %Hcontr. 
+      iDestruct "Hl'" as (ρ') "[Hstate Hl']". 
+      iDestruct (sts_full_state_std with "Hfull Hstate") as %Hcontr.
+      apply not_elem_of_dom in Hnone1. 
+      rewrite Hcontr in Hnone1. done.
     }
     (* if not, we need to allocate a new saved pred using φ, 
        and extend R with l := pred *)
     iMod (saved_pred_alloc φ) as (γpred) "#Hφ'".
-    iMod (own_update _ _ (● (<[l:=to_agree (γpred,_)]> M) ⋅ ◯ ({[l:=to_agree (γpred,_)]}))
+    iMod (own_update _ _ (● (<[l:=to_agree (γpred,_)]> (to_agree <$> M : relUR)) ⋅ ◯ ({[l:=to_agree (γpred,_)]}))
             with "Hγrel") as "[HR #Hγrel]". 
     { apply auth_update_alloc.
-      by apply alloc_singleton_local_update. 
+      apply (alloc_singleton_local_update (to_agree <$> M)); last done.
+      rewrite lookup_fmap. rewrite HRl. done. 
     }
-    iApply fupd_frame_l. iSplitL "HR Hpreds Hl".
-    - iExists _. iFrame "HR #".
-      iApply big_sepM_insert; auto.
-      iFrame. iExists γpred,v,_,φ. iSplitR;[auto|]. iFrame "∗ #". done. 
+    (* we also need to extend the World with a new temporary region *)
+    iMod (sts_alloc_std_i W (countable.encode l) Temporary
+            with "[] Hfull") as "(Hfull & Hstate)"; auto.     
+    apply (related_sts_pub_world_fresh W l Temporary) in Hnone1 as Hrelated; auto.
+    iDestruct (region_map_monotone $! Hrelated with "Hpreds") as "Hpreds'".
+    iModIntro. rewrite bi.sep_exist_r. iExists _.
+    rewrite -fmap_insert. 
+    iFrame "HR". iFrame.
+    iSplitL;[iSplitR|].
+    - iPureIntro. apply dom_equal_insert; auto. 
+    - iApply big_sepM_insert; auto.
+      iFrame. iExists Temporary.
+      iFrame. iExists γpred,v,_,φ. iSplitR;[auto|]. iFrame "∗ #".
+      iSplitR;[done|].
+      rewrite Hpwl. iFrame "#".
+      iNext. iApply "Hmono"; eauto.
     - iExists γpred. iFrame "#".
       rewrite REL_eq /REL_def. 
       done. 
   Qed.
 
-  Definition open_region_def (a : Addr) (W : WORLD) : iProp Σ :=
-    (∃ M, RELS M ∗
-    [∗ map] l↦γ ∈ (delete a M), ∃ γpred v p φ, ⌜γ = to_agree (γpred,p)⌝
-                                  ∗ ⌜p ≠ O⌝                           
-                                  ∗ (l ↦ₐ[p] v)
-                                  ∗ future_mono φ
-                                  ∗ saved_pred_own γpred φ
-                                  ∗ ▷ φ (W,v))%I.
-  Definition open_region_aux : { x | x = @open_region_def }. by eexists. Qed.
-  Definition open_region := proj1_sig open_region_aux.
-  Definition open_region_eq : @open_region = @open_region_def := proj2_sig open_region_aux.
-
-  Lemma region_open W l p φ :
-    rel l p φ ∗ region W -∗ ∃ v, open_region l W
-                               ∗ (l ↦ₐ[p] v)
-                               ∗ ⌜p ≠ O⌝
-                               ∗ ▷ future_mono φ
-                               ∗ ▷ φ (W,v).
+  Lemma extend_region_temp_nwl E W l p v φ `{∀ W v, Persistent (φ (W,v))}:
+     p ≠ O →
+     (countable.encode l) ∉ dom (gset positive) (std_sta W) →
+     (countable.encode l) ∉ dom (gset positive) (std_rel W) →
+     (pwl p) = false →
+     (future_priv_mono φ v →
+     sts_full_world sts_std W -∗ region W -∗ l ↦ₐ[p] v -∗ φ (W,v) ={E}=∗ region (<s[l := Temporary, (Rpub,Rpriv) ]s>W)
+                                                              ∗ rel l p φ
+                                                              ∗ sts_full_world sts_std (<s[l := Temporary, (Rpub,Rpriv)]s>W))%I.
   Proof.
-    iIntros "[Hrel Hreg]".
-    rewrite rel_eq region_eq /rel_def /region_def REL_eq RELS_eq /REL_def /RELS_def. 
-    iDestruct "Hrel" as (γpred) "#[Hγpred Hφ]".
-    iDestruct "Hreg" as (M) "(HM & Hpreds)". 
+    iIntros (Hpne Hnone1 Hnone2 Hpwl) "#Hmono Hfull Hreg Hl #Hφ".
+    rewrite region_eq rel_eq /region_def /rel_def.
+    iDestruct "Hreg" as (M) "(Hγrel & % & Hpreds)".
+    rewrite RELS_eq /RELS_def. 
+    (* destruct on M !! l *)
+    destruct (M !! l) eqn:HRl.
+    { (* The location is not in the map *)
+      iDestruct (big_sepM_delete _ _ _ _ HRl with "Hpreds") as "[Hl' _]".
+      iDestruct "Hl'" as (ρ') "[Hstate Hl']". 
+      iDestruct (sts_full_state_std with "Hfull Hstate") as %Hcontr.
+      apply not_elem_of_dom in Hnone1. 
+      rewrite Hcontr in Hnone1. done.
+    }
+    (* if not, we need to allocate a new saved pred using φ, 
+       and extend R with l := pred *)
+    iMod (saved_pred_alloc φ) as (γpred) "#Hφ'".
+    iMod (own_update _ _ (● (<[l:=to_agree (γpred,_)]> (to_agree <$> M : relUR)) ⋅ ◯ ({[l:=to_agree (γpred,_)]}))
+            with "Hγrel") as "[HR #Hγrel]". 
+    { apply auth_update_alloc.
+      apply (alloc_singleton_local_update (to_agree <$> M)); last done.
+      rewrite lookup_fmap. rewrite HRl. done. 
+    }
+    (* we also need to extend the World with a new temporary region *)
+    iMod (sts_alloc_std_i W (countable.encode l) Temporary
+            with "[] Hfull") as "(Hfull & Hstate)"; auto.     
+    apply (related_sts_pub_world_fresh W l Temporary) in Hnone1 as Hrelated; auto. 
+    iDestruct (region_map_monotone $! Hrelated with "Hpreds") as "Hpreds'".
+    iModIntro. rewrite bi.sep_exist_r. iExists _.
+    rewrite -fmap_insert. 
+    iFrame "HR". iFrame.
+    iSplitL;[iSplitR|].
+    - iPureIntro. apply dom_equal_insert; auto. 
+    - iApply big_sepM_insert; auto.
+      iFrame. iExists Temporary.
+      iFrame. iExists γpred,v,_,φ. iSplitR;[auto|]. iFrame "∗ #".
+      iSplitR;[done|].
+      rewrite Hpwl. iFrame "#".
+      iNext. iApply "Hmono"; eauto.
+      iPureIntro. by apply related_sts_pub_priv_world. 
+    - iExists γpred. iFrame "#".
+      rewrite REL_eq /REL_def. 
+      done. 
+  Qed.
+
+  Lemma extend_region_perm E W l p v φ `{∀ W v, Persistent (φ (W,v))}:
+     p ≠ O →
+     (countable.encode l) ∉ dom (gset positive) (std_sta W) →
+     (countable.encode l) ∉ dom (gset positive) (std_rel W) →
+     (future_priv_mono φ v →
+     sts_full_world sts_std W -∗ region W -∗ l ↦ₐ[p] v -∗ φ (W,v) ={E}=∗ region (<s[l := Permanent, (Rpub,Rpriv) ]s>W)
+                                                              ∗ rel l p φ
+                                                              ∗ sts_full_world sts_std (<s[l := Permanent, (Rpub,Rpriv)]s>W))%I.
+  Proof.
+    iIntros (Hpne Hnone1 Hnone2) "#Hmono Hfull Hreg Hl #Hφ".
+    rewrite region_eq rel_eq /region_def /rel_def.
+    iDestruct "Hreg" as (M) "(Hγrel & % & Hpreds)".
+    rewrite RELS_eq /RELS_def. 
+    (* destruct on M !! l *)
+    destruct (M !! l) eqn:HRl.
+    { (* The location is not in the map *)
+      iDestruct (big_sepM_delete _ _ _ _ HRl with "Hpreds") as "[Hl' _]".
+      iDestruct "Hl'" as (ρ') "[Hstate Hl']". 
+      iDestruct (sts_full_state_std with "Hfull Hstate") as %Hcontr.
+      apply not_elem_of_dom in Hnone1. 
+      rewrite Hcontr in Hnone1. done.
+    }
+    (* if not, we need to allocate a new saved pred using φ, 
+       and extend R with l := pred *)
+    iMod (saved_pred_alloc φ) as (γpred) "#Hφ'".
+    iMod (own_update _ _ (● (<[l:=to_agree (γpred,_)]> (to_agree <$> M : relUR)) ⋅ ◯ ({[l:=to_agree (γpred,_)]}))
+            with "Hγrel") as "[HR #Hγrel]". 
+    { apply auth_update_alloc.
+      apply (alloc_singleton_local_update (to_agree <$> M)); last done.
+      rewrite lookup_fmap. rewrite HRl. done. 
+    }
+    (* we also need to extend the World with a new temporary region *)
+    iMod (sts_alloc_std_i W (countable.encode l) Permanent
+            with "[] Hfull") as "(Hfull & Hstate)"; auto.     
+    apply (related_sts_pub_world_fresh W l Permanent) in Hnone1 as Hrelated; auto. 
+    iDestruct (region_map_monotone $! Hrelated with "Hpreds") as "Hpreds'".
+    iModIntro. rewrite bi.sep_exist_r. iExists _.
+    rewrite -fmap_insert. 
+    iFrame "HR". iFrame.
+    iSplitL;[iSplitR|].
+    - iPureIntro. apply dom_equal_insert; auto. 
+    - iApply big_sepM_insert; auto.
+      iFrame. iExists Permanent.
+      iFrame. iExists γpred,v,_,φ. iSplitR;[auto|]. iFrame "∗ #".
+      iSplitR;[done|].
+      iNext. iApply "Hmono"; eauto.
+      iPureIntro. by apply related_sts_pub_priv_world. 
+    - iExists γpred. iFrame "#".
+      rewrite REL_eq /REL_def. 
+      done. 
+  Qed.
+
+  Lemma region_open_temp_pwl W l p φ :
+    (std_sta W) !! (countable.encode l) = Some (countable.encode Temporary) →
+    pwl p = true →
+    rel l p φ ∗ region W ∗ sts_full_world sts_std W -∗
+        ∃ v, open_region l W
+           ∗ sts_full_world sts_std W
+           ∗ sts_state_std (countable.encode l) Temporary
+           ∗ l ↦ₐ[p] v
+           ∗ ⌜p ≠ O⌝
+           ∗ ▷ future_pub_mono φ v
+           ∗ ▷ φ (W,v).
+  Proof.
+    iIntros (Htemp Hpwl) "(Hrel & Hreg & Hfull)".
+    rewrite rel_eq region_eq /rel_def /region_def REL_eq RELS_eq /REL_def /RELS_def /region_map_def. 
+    iDestruct "Hrel" as (γpred) "#(Hγpred & Hφ)".
+    iDestruct "Hreg" as (M) "(HM & % & Hpreds)". 
     (* assert that γrel = γrel' *)
-    iDestruct (reg_in γrel M with "[$HM $Hγpred]") as %HMeq.
-    rewrite HMeq big_sepM_insert; [|by rewrite lookup_delete]. 
+    iDestruct (reg_in γrel (M) with "[$HM $Hγpred]") as %HMeq.
+    rewrite HMeq big_sepM_insert; [|by rewrite lookup_delete].
     iDestruct "Hpreds" as "[Hl Hpreds]".
-    iDestruct "Hl" as (γpred' v p' φ') "(% & % & Hl & #Hmono & #Hφ' & Hφv)".  
-    inversion H2; subst.
+    iDestruct "Hl" as (ρ) "[Hstate Hl]". destruct ρ. 
+    2: { iDestruct (sts_full_state_std with "Hfull Hstate") as %Hcontr.
+         rewrite Htemp in Hcontr. inversion Hcontr. apply countable.encode_inj in H5. done. }
+    2: { iDestruct (sts_full_state_std with "Hfull Hstate") as %Hcontr.
+         rewrite Htemp in Hcontr. inversion Hcontr. apply countable.encode_inj in H5. done. }
+    iDestruct "Hl" as (γpred' v p' φ') "(% & % & Hl & Hmono & #Hφ' & Hφv)".  
+    inversion H4; subst. rewrite Hpwl. iDestruct "Hmono" as "#Hmono".  
     iDestruct (saved_pred_agree _ _ _ (W,v) with "Hφ Hφ'") as "#Hφeq".
     iExists v. iFrame.
     iSplitR "Hφv". 
     - rewrite open_region_eq /open_region_def.
-      iExists _. rewrite RELS_eq -HMeq. iFrame "∗ #". 
+      iExists _. rewrite RELS_eq /RELS_def -HMeq. iFrame "∗ #".
+      auto. 
     - iSplitR;[auto|]. iSplitR. 
-      + rewrite /future_mono.
+      + rewrite /future_pub_mono.
         iApply later_intuitionistically_2. iAlways.
         repeat (iApply later_forall_2; iIntros (?)).
-        iDestruct (saved_pred_agree _ _ _ (a0,a1) with "Hφ Hφ'") as "#Hφeq'".
-        iDestruct (saved_pred_agree _ _ _ (a,a1) with "Hφ Hφ'") as "#Hφeq''".
+        iDestruct (saved_pred_agree _ _ _ (a,v) with "Hφ Hφ'") as "#Hφeq'".
+        iDestruct (saved_pred_agree _ _ _ (a0,v) with "Hφ Hφ'") as "#Hφeq''".
+        iNext. iIntros (Hrel) "Hφw".
+        iRewrite ("Hφeq''"). 
+        iApply "Hmono"; eauto.
+        iRewrite -("Hφeq'"). iFrame. 
+      + iNext. iRewrite "Hφeq". iFrame "∗ #".
+  Qed.
+
+  Lemma region_open_temp_nwl W l p φ :
+    (std_sta W) !! (countable.encode l) = Some (countable.encode Temporary) →
+    pwl p = false →
+    rel l p φ ∗ region W ∗ sts_full_world sts_std W -∗
+        ∃ v, open_region l W
+           ∗ sts_full_world sts_std W
+           ∗ sts_state_std (countable.encode l) Temporary
+           ∗ l ↦ₐ[p] v
+           ∗ ⌜p ≠ O⌝
+           ∗ ▷ future_priv_mono φ v
+           ∗ ▷ φ (W,v).
+  Proof.
+    iIntros (Htemp Hpwl) "(Hrel & Hreg & Hfull)".
+    rewrite rel_eq region_eq /rel_def /region_def REL_eq RELS_eq /REL_def /RELS_def /region_map_def. 
+    iDestruct "Hrel" as (γpred) "#[Hγpred Hφ]".
+    iDestruct "Hreg" as (M) "(HM & % & Hpreds)". 
+    (* assert that γrel = γrel' *)
+    iDestruct (reg_in γrel M with "[$HM $Hγpred]") as %HMeq.
+    rewrite HMeq big_sepM_insert; [|by rewrite lookup_delete].
+    iDestruct "Hpreds" as "[Hl Hpreds]".
+    iDestruct "Hl" as (ρ) "[Hstate Hl]". destruct ρ. 
+    2: { iDestruct (sts_full_state_std with "Hfull Hstate") as %Hcontr.
+         rewrite Htemp in Hcontr. inversion Hcontr. apply countable.encode_inj in H5. done. }
+    2: { iDestruct (sts_full_state_std with "Hfull Hstate") as %Hcontr.
+         rewrite Htemp in Hcontr. inversion Hcontr. apply countable.encode_inj in H5. done. }
+    iDestruct "Hl" as (γpred' v p' φ') "(% & % & Hl & Hmono & #Hφ' & Hφv)".  
+    inversion H4; subst. rewrite Hpwl. iDestruct "Hmono" as "#Hmono".  
+    iDestruct (saved_pred_agree _ _ _ (W,v) with "Hφ Hφ'") as "#Hφeq".
+    iExists v. iFrame.
+    iSplitR "Hφv". 
+    - rewrite open_region_eq /open_region_def.
+      iExists _. rewrite RELS_eq /RELS_def -HMeq. iFrame "∗ #".
+      auto. 
+    - iSplitR;[auto|]. iSplitR. 
+      + rewrite /future_pub_mono.
+        iApply later_intuitionistically_2. iAlways.
+        repeat (iApply later_forall_2; iIntros (?)).
+        iDestruct (saved_pred_agree _ _ _ (a,v) with "Hφ Hφ'") as "#Hφeq'".
+        iDestruct (saved_pred_agree _ _ _ (a0,v) with "Hφ Hφ'") as "#Hφeq''".
+        iNext. iIntros (Hrel) "Hφw".
+        iRewrite ("Hφeq''"). 
+        iApply "Hmono"; eauto.
+        iRewrite -("Hφeq'"). iFrame. 
+      + iNext. iRewrite "Hφeq". iFrame "∗ #".
+  Qed.
+
+  Lemma region_open_perm W l p φ :
+    (std_sta W) !! (countable.encode l) = Some (countable.encode Permanent) →
+    rel l p φ ∗ region W ∗ sts_full_world sts_std W -∗
+        ∃ v, open_region l W
+           ∗ sts_full_world sts_std W
+           ∗ sts_state_std (countable.encode l) Permanent              
+           ∗ l ↦ₐ[p] v
+           ∗ ⌜p ≠ O⌝
+           ∗ ▷ future_priv_mono φ v
+           ∗ ▷ φ (W,v).
+  Proof.
+    iIntros (Htemp) "(Hrel & Hreg & Hfull)".
+    rewrite rel_eq region_eq /rel_def /region_def REL_eq RELS_eq /REL_def /RELS_def /region_map_def. 
+    iDestruct "Hrel" as (γpred) "#[Hγpred Hφ]".
+    iDestruct "Hreg" as (M) "(HM & % & Hpreds)". 
+    (* assert that γrel = γrel' *)
+    iDestruct (reg_in γrel M with "[$HM $Hγpred]") as %HMeq.
+    rewrite HMeq big_sepM_insert; [|by rewrite lookup_delete].
+    iDestruct "Hpreds" as "[Hl Hpreds]".
+    iDestruct "Hl" as (ρ) "[Hstate Hl]". destruct ρ. 
+    1: { iDestruct (sts_full_state_std with "Hfull Hstate") as %Hcontr.
+         rewrite Htemp in Hcontr. inversion Hcontr. apply countable.encode_inj in H5. done. }
+    2: { iDestruct (sts_full_state_std with "Hfull Hstate") as %Hcontr.
+         rewrite Htemp in Hcontr. inversion Hcontr. apply countable.encode_inj in H5. done. }
+    iDestruct "Hl" as (γpred' v p' φ') "(% & % & Hl & #Hmono & #Hφ' & Hφv)".  
+    inversion H4; subst.
+    iDestruct (saved_pred_agree _ _ _ (W,v) with "Hφ Hφ'") as "#Hφeq".
+    iExists v. iFrame.
+    iSplitR "Hφv". 
+    - rewrite open_region_eq /open_region_def.
+      iExists _. rewrite RELS_eq /RELS_def -HMeq. iFrame "∗ #".
+      auto. 
+    - iSplitR;[auto|]. iSplitR. 
+      + rewrite /future_priv_mono.
+        iApply later_intuitionistically_2. iAlways.
+        repeat (iApply later_forall_2; iIntros (?)).
+        iDestruct (saved_pred_agree _ _ _ (a0,v) with "Hφ Hφ'") as "#Hφeq'".
+        iDestruct (saved_pred_agree _ _ _ (a,v) with "Hφ Hφ'") as "#Hφeq''".
         iNext. iIntros (Hrel) "Hφw".
         iRewrite ("Hφeq'"). 
         iApply "Hmono"; eauto.
@@ -185,23 +640,657 @@ Section heap.
       + iNext. iRewrite "Hφeq". iFrame "∗ #".
   Qed.
 
-  Lemma region_close W l φ p v :
-    open_region l W ∗ l ↦ₐ[p] v ∗ ⌜p ≠ O⌝ ∗ future_mono φ ∗ ▷ φ (W,v) ∗ rel l p φ
+  (* Closing the region without updating the world *)
+  Lemma region_close_temp_pwl W l φ p v :
+    pwl p = true →
+    sts_state_std (countable.encode l) Temporary
+                  ∗ open_region l W ∗ l ↦ₐ[p] v ∗ ⌜p ≠ O⌝ ∗ future_pub_mono φ v ∗ ▷ φ (W,v) ∗ rel l p φ
     -∗ region W.
   Proof.
     rewrite open_region_eq rel_eq region_eq /open_region_def /rel_def /region_def
             REL_eq RELS_eq /RELS_def /REL_def.
-    iIntros "(Hreg_open & Hl & % & #Hmono & Hφ & #Hrel)".
+    iIntros (Hpwl) "(Hstate & Hreg_open & Hl & % & #Hmono & Hφ & #Hrel)".
     iDestruct "Hrel" as (γpred) "#[Hγpred Hφ_saved]".
-    iDestruct "Hreg_open" as (M) "(HM & Hpreds)".
+    iDestruct "Hreg_open" as (M) "(HM & % & Hpreds)".
     iDestruct (big_sepM_insert _ (delete l M) l with "[-HM]") as "test";
       first by rewrite lookup_delete.
-    { iFrame. iExists _,_,_,_. iFrame "∗ #". (iSplitR;[eauto|]). done. }
+    { iFrame. iExists Temporary. iFrame. iExists _,_,p,_. rewrite Hpwl. iFrame "∗ #". (iSplitR;[eauto|]). done. }
     iExists _. iFrame "∗ #".
     iDestruct (reg_in γrel M with "[$HM $Hγpred]") as %HMeq.
-    rewrite -HMeq. iFrame.
-  Qed.  
+    rewrite -HMeq. iFrame. auto. 
+  Qed.
+
+  Lemma region_close_temp_nwl W l φ p v :
+    pwl p = false →
+    sts_state_std (countable.encode l) Temporary
+                  ∗ open_region l W ∗ l ↦ₐ[p] v ∗ ⌜p ≠ O⌝ ∗ future_priv_mono φ v ∗ ▷ φ (W,v) ∗ rel l p φ
+    -∗ region W.
+  Proof.
+    rewrite open_region_eq rel_eq region_eq /open_region_def /rel_def /region_def
+            REL_eq RELS_eq /RELS_def /REL_def.
+    iIntros (Hpwl) "(Hstate & Hreg_open & Hl & % & #Hmono & Hφ & #Hrel)".
+    iDestruct "Hrel" as (γpred) "#[Hγpred Hφ_saved]".
+    iDestruct "Hreg_open" as (M) "(HM & % & Hpreds)".
+    iDestruct (big_sepM_insert _ (delete l M) l with "[-HM]") as "test";
+      first by rewrite lookup_delete.
+    { iFrame. iExists Temporary. iFrame. iExists _,_,p,_. rewrite Hpwl. iFrame "∗ #". (iSplitR;[eauto|]). done. }
+    iExists _. iFrame "∗ #".
+    iDestruct (reg_in γrel M with "[$HM $Hγpred]") as %HMeq.
+    rewrite -HMeq. iFrame. auto. 
+  Qed.
+
+  Lemma region_close_perm W l φ p v :
+    sts_state_std (countable.encode l) Permanent
+                  ∗ open_region l W ∗ l ↦ₐ[p] v ∗ ⌜p ≠ O⌝ ∗ future_priv_mono φ v ∗ ▷ φ (W,v) ∗ rel l p φ
+    -∗ region W.
+  Proof.
+    rewrite open_region_eq rel_eq region_eq /open_region_def /rel_def /region_def
+            REL_eq RELS_eq /RELS_def /REL_def.
+    iIntros "(Hstate & Hreg_open & Hl & % & #Hmono & Hφ & #Hrel)".
+    iDestruct "Hrel" as (γpred) "#[Hγpred Hφ_saved]".
+    iDestruct "Hreg_open" as (M) "(HM & % & Hpreds)".
+    iDestruct (big_sepM_insert _ (delete l M) l with "[-HM]") as "test";
+      first by rewrite lookup_delete.
+    { iFrame. iExists Permanent. iFrame. iExists _,_,_,_. iFrame "∗ #". (iSplitR;[eauto|]). done. }
+    iExists _. iFrame "∗ #".
+    iDestruct (reg_in γrel M with "[$HM $Hγpred]") as %HMeq.
+    rewrite -HMeq. iFrame. auto. 
+  Qed.
+
+  (* Next we need to define revocation of memory *)
+
+  (* Revocation only changes the states of the standard STS collection *)
+  Definition revoke_std_sta : STS_states → STS_states :=
+    fmap (λ v, if ((countable.encode Temporary) =? v)%positive then countable.encode Revoked else v
+         (* match countable.decode v with *)
+         (* | Some Temporary => countable.encode Revoked *)
+         (* | _ => v *)
+         (* end *) ). 
+  Definition revoke W : WORLD := ((revoke_std_sta (std_sta W),std_rel W), loc W).
+
+  (* A weaker revocation which only revokes elements from a list *)
+  Fixpoint revoke_list_std_sta (l : list positive) (fs : STS_states) : STS_states :=
+    match l with
+    | [] => fs
+    | i :: l' => match fs !! i with
+               | Some j => if ((countable.encode Temporary) =? j)%positive
+                          then <[i := countable.encode Revoked]> (revoke_list_std_sta l' fs)
+                          else (revoke_list_std_sta l' fs)
+               (* match countable.decode j with *)
+               (* | Some Temporary => <[i := countable.encode Revoked]> (revoke_list_std_sta l' fs) *)
+               (* | _ => (revoke_list_std_sta l' fs) *)
+               (* end *)
+               | None => (revoke_list_std_sta l' fs)
+               end
+    end.
+  Definition revoke_list l W : WORLD := ((revoke_list_std_sta l (std_sta W),std_rel W), loc W).
+
+  Lemma revoke_list_swap Wstd_sta l a b :
+    revoke_list_std_sta (a :: b :: l) Wstd_sta = revoke_list_std_sta (b :: a :: l) Wstd_sta.
+  Proof.
+    destruct (decide (a = b)).
+    - subst. done.
+    - simpl. destruct (Wstd_sta !! b) eqn:Hb,(Wstd_sta !! a) eqn:Ha; try reflexivity.
+      destruct (countable.encode Temporary =? p0)%positive eqn:Hp0,
+               (countable.encode Temporary =? p)%positive eqn:Hp; try reflexivity. 
+      rewrite insert_commute; auto.
+  Qed.
+
+  Lemma revoke_list_swap_middle Wstd_sta l1 l2 a :
+    revoke_list_std_sta (l1 ++ a :: l2) Wstd_sta = revoke_list_std_sta (a :: l1 ++ l2) Wstd_sta.
+  Proof.
+    induction l1.
+    - done.
+    - assert (a :: (a0 :: l1) ++ l2 = a :: a0 :: l1 ++ l2) as -> ; auto.
+      assert ((a0 :: l1) ++ a :: l2 = a0 :: l1 ++ a :: l2) as ->; auto. 
+      rewrite revoke_list_swap. simpl. rewrite IHl1. done.
+  Qed.
+
+  Lemma revoke_list_permutation Wstd_sta l1 l2 :
+    l1 ≡ₚ l2 →
+    revoke_list_std_sta l1 Wstd_sta = revoke_list_std_sta l2 Wstd_sta.
+  Proof.
+    intros Hperm. 
+    induction Hperm using Permutation_ind.
+    - done.
+    - simpl. destruct (Wstd_sta !! x); auto.
+      destruct (countable.encode Temporary =? p)%positive; auto.
+      f_equiv. done.
+    - by rewrite revoke_list_swap.
+    - by rewrite IHHperm1 IHHperm2.
+  Qed.
+
+  Lemma revoke_list_insert_insert i x y l m :
+    <[i:=x]> (revoke_list_std_sta l (<[i:=y]> m)) = <[i:=x]> (revoke_list_std_sta l m).
+  Proof.
+    induction l. 
+    - simpl. rewrite insert_insert. done.
+    - simpl. destruct (m !! a) eqn:Hsome.
+      + destruct (decide (a = i)).
+        * subst. rewrite lookup_insert. 
+          destruct (countable.encode Temporary =? y)%positive,(countable.encode Temporary =? p)%positive;
+            try rewrite insert_insert; auto.
+          rewrite IHl. rewrite insert_insert;auto.
+        * rewrite lookup_insert_ne;auto. rewrite Hsome.
+          destruct (countable.encode Temporary =? p)%positive;auto.
+          do 2 (rewrite (insert_commute _ i a);auto). 
+          f_equiv. done.
+      + destruct (decide (a = i)).
+        * subst. rewrite lookup_insert.
+          destruct (countable.encode Temporary =? y)%positive; auto.
+          rewrite insert_insert. done.
+        * rewrite lookup_insert_ne;auto. rewrite Hsome.
+          done. 
+  Qed.
+
+  Lemma revoke_list_not_elem_of i x l m :
+    i ∉ l →
+    <[i:=x]> (revoke_list_std_sta l m) = revoke_list_std_sta l (<[i:=x]> m).
+  Proof.
+    induction l;intros Hnin.
+    - done.
+    - apply not_elem_of_cons in Hnin as [Hneq Hnin]. 
+      simpl. destruct (m !! a) eqn:Hsome.
+      + rewrite lookup_insert_ne;auto. rewrite Hsome.
+        destruct (countable.encode Temporary =? p)%positive; auto.
+        rewrite insert_commute;auto. f_equiv. auto.
+      + rewrite lookup_insert_ne;auto. rewrite Hsome.
+        auto.
+  Qed.
+
+  Lemma revoke_list_not_elem_of_lookup i l m :
+    i ∉ l →
+    (revoke_list_std_sta l m) !! i = m !! i.
+  Proof.
+    induction l; intros Hnin. 
+    - done.
+    - apply not_elem_of_cons in Hnin as [Hneq Hnin]. 
+      simpl. destruct (m !! a) eqn:Hsome.
+      + destruct (countable.encode Temporary =? p)%positive; auto.
+        rewrite lookup_insert_ne; auto. 
+      + auto.
+  Qed.
+    
+  Lemma revoke_list_dom W :
+    revoke W = revoke_list (map_to_list W.1.1).*1 W.
+  Proof.
+    destruct W as [ [Wstd_sta Wstd_rel] Wloc]. 
+    induction Wstd_sta using map_ind.
+    - rewrite /revoke /revoke_std_sta /=. 
+        by rewrite fmap_empty map_to_list_empty /revoke_list /std_sta /std_rel /=.
+    - rewrite /revoke /revoke_std_sta /=.
+      rewrite fmap_insert.
+      apply map_to_list_insert with m i x in H3 as Hperm.
+      apply (fmap_Permutation fst) in Hperm. 
+      rewrite /revoke_list (revoke_list_permutation _ _ ((i, x) :: map_to_list m).*1); auto.
+      rewrite /= lookup_insert.
+      destruct (countable.encode Temporary =? x)%positive; auto.
+      + rewrite /std_rel /std_sta /=. 
+        rewrite /revoke /revoke_list /revoke_std_sta /std_sta /std_rel /= in IHWstd_sta.
+        inversion IHWstd_sta.
+        do 2 f_equiv. 
+        rewrite revoke_list_insert_insert. repeat f_equiv. auto.
+      + rewrite /std_rel /std_sta /=. do 2 f_equiv.
+        rewrite /revoke /revoke_list /revoke_std_sta /std_sta /std_rel /= in IHWstd_sta.
+        inversion IHWstd_sta. rewrite H5.
+        apply revoke_list_not_elem_of.
+        intros Hcontr. apply (elem_of_list_fmap_2 fst) in Hcontr.
+        destruct Hcontr as [ [y1 y2] [Hy Hyin] ]. subst.
+        apply elem_of_map_to_list in Hyin. simpl in *. congruence.
+  Qed.
+
+  Lemma map_to_list_fst {A B : Type} `{EqDecision A, Countable A} (m : gmap A B) i :
+    i ∈ (map_to_list m).*1 ↔ (∃ x, (i,x) ∈ (map_to_list m)).
+  Proof.
+    split.
+    - intros Hi.
+      destruct (m !! i) eqn:Hsome.
+      + exists b. by apply elem_of_map_to_list.
+      + apply not_elem_of_list_to_map in Hi; [done|].
+          by rewrite list_to_map_to_list.
+    - intros [x Hix].
+      apply elem_of_list_fmap.
+      exists (i,x). auto. 
+  Qed.       
+
+  Lemma revoke_list_lookup_Some Wstd_sta l (i : positive) :
+    is_Some (Wstd_sta !! i) ↔ is_Some ((revoke_list_std_sta l Wstd_sta) !! i). 
+  Proof.
+    split.
+    - induction l.
+      + done.
+      + intros [x Hx]. 
+      simpl.
+      destruct (Wstd_sta !! a);[|apply IHl;eauto].
+      destruct (countable.encode Temporary =? p)%positive;[|apply IHl;eauto].
+      destruct (decide (a = i)).
+        * subst. rewrite lookup_insert. eauto.
+        * rewrite lookup_insert_ne;eauto. 
+    - induction l.
+      + done.
+      + intros [x Hx].
+        simpl in Hx.
+        destruct (Wstd_sta !! a) eqn:Hsome;eauto. 
+        destruct (countable.encode Temporary =? p)%positive;[|apply IHl;eauto].
+        destruct (decide (a = i)).
+        * subst. eauto. 
+        * rewrite lookup_insert_ne in Hx;eauto. 
+  Qed.
+
+  Lemma revoke_lookup_Some W (i : positive) :
+    is_Some ((std_sta W) !! i) ↔ is_Some ((std_sta (revoke W)) !! i).
+  Proof.
+    rewrite revoke_list_dom.
+    apply revoke_list_lookup_Some. 
+  Qed. 
+
+  Lemma revoke_list_nin Wstd_sta (l : list positive) (i : positive) :
+    i ∉ l → (revoke_list_std_sta l Wstd_sta) !! i = Wstd_sta !! i.
+  Proof.
+    intros Hnin.
+    induction l.
+    - done.
+    - apply not_elem_of_cons in Hnin as [Hneq Hnin].
+      simpl. destruct (Wstd_sta !! a); auto.
+      destruct  (countable.encode Temporary =? p)%positive;auto. 
+      rewrite lookup_insert_ne; auto.
+  Qed. 
+      
+  Lemma revoke_list_lookup_Temp (Wstd_sta : STS_states) (l : list positive) (i : positive) :
+    (Wstd_sta !! i = Some (countable.encode Temporary)) →
+    (revoke_list_std_sta (i :: l) Wstd_sta) !! i = Some (countable.encode Revoked). 
+  Proof.
+    intros Hp.
+    rewrite /= Hp Positive_as_OT.eqb_refl. 
+    apply lookup_insert. 
+  Qed.
+
+  Lemma revoke_list_lookup_middle_Temp (Wstd_sta : STS_states) (l : list positive) (i : positive) :
+    i ∈ l →
+    (Wstd_sta !! i = Some (countable.encode Temporary)) →
+    (revoke_list_std_sta l Wstd_sta) !! i = Some (countable.encode Revoked). 
+  Proof.
+    intros Hin Hp.
+    apply elem_of_list_split in Hin as [l1 [l2 ->] ].
+    rewrite revoke_list_swap_middle.
+    by apply revoke_list_lookup_Temp. 
+  Qed.
+
+  Lemma revoke_list_lookup_Revoked (Wstd_sta : STS_states) (l : list positive) (i : positive) :
+    (Wstd_sta !! i = Some (countable.encode Revoked)) →
+    (revoke_list_std_sta (i :: l) Wstd_sta) !! i = Some (countable.encode Revoked). 
+  Proof.
+    intros Hp.
+    induction l.
+    - rewrite /= Hp.
+      destruct (countable.encode Temporary =? countable.encode Revoked)%positive; [|done]. apply lookup_insert. 
+    - rewrite revoke_list_swap /=.
+      destruct (Wstd_sta !! a); auto.
+      destruct (countable.encode Temporary =? p)%positive; auto. 
+      rewrite Hp.
+      destruct (decide (a = i)).
+      + subst. apply lookup_insert.
+      + rewrite lookup_insert_ne;auto.
+        rewrite /= Hp in IHl.
+        destruct (countable.encode Temporary =? countable.encode Revoked)%positive; auto. 
+  Qed.
+
+  Lemma revoke_list_lookup_Perm (Wstd_sta : STS_states) (l : list positive) (i : positive) :
+    i ∉ l →
+    (Wstd_sta !! i = Some (countable.encode Permanent)) →
+    (revoke_list_std_sta (i :: l) Wstd_sta) !! i = Some (countable.encode Permanent). 
+  Proof.
+    induction l.
+    - intros Hin Hp.
+      rewrite /= Hp. 
+      destruct (countable.encode Temporary =? countable.encode Permanent)%positive eqn:Hcontr; [|done].
+      apply Positive_as_OT.eqb_eq,encode_inj in Hcontr; inversion Hcontr. 
+    - intros Hin Hp.
+      apply not_elem_of_cons in Hin as [Hneq Hin]. 
+      rewrite revoke_list_swap. 
+      rewrite /=.
+      destruct (Wstd_sta !! a).
+      + rewrite Hp. destruct (countable.encode Temporary =? p)%positive.
+        * destruct (countable.encode Temporary =? countable.encode Permanent)%positive eqn:Hcontr; [|].
+          apply Positive_as_OT.eqb_eq,encode_inj in Hcontr; inversion Hcontr.
+          rewrite lookup_insert_ne;auto.
+          specialize (IHl Hin Hp). 
+          by rewrite /= Hp Hcontr in IHl. 
+        * destruct (countable.encode Temporary =? countable.encode Permanent)%positive eqn:Hcontr; [|].
+          apply Positive_as_OT.eqb_eq,encode_inj in Hcontr; inversion Hcontr.
+          specialize (IHl Hin Hp). 
+          by rewrite /= Hp Hcontr in IHl. 
+      + rewrite Hp. 
+        destruct (countable.encode Temporary =? countable.encode Permanent)%positive eqn:Hcontr; [|].
+        apply Positive_as_OT.eqb_eq,encode_inj in Hcontr; inversion Hcontr.
+        specialize (IHl Hin Hp). 
+          by rewrite /= Hp Hcontr in IHl. 
+  Qed.
+
+  Lemma revoke_list_lookup_None (Wstd_sta : STS_states) (l : list positive) (i : positive) :
+    i ∉ l →
+    (Wstd_sta !! i = None →
+     (revoke_list_std_sta (i :: l) Wstd_sta) !! i = None).
+  Proof.
+    intros Hin Hnone.
+    induction l. 
+    - by rewrite /= Hnone. 
+    - rewrite revoke_list_swap.
+      apply not_elem_of_cons in Hin as [Hneq Hin]. 
+      rewrite /= Hnone in IHl.
+      rewrite /= Hnone.
+      destruct (Wstd_sta !! a); auto.
+      destruct (countable.encode Temporary =? p)%positive; auto. 
+      rewrite lookup_insert_ne;auto.
+  Qed. 
+    
+  Lemma map_size_insert_Some {K A} `{EqDecision K, Countable K} i x (m : gmap K A) :
+    is_Some(m !! i) → size (<[i:=x]> m) = (size m).
+  Proof. induction m using map_ind.
+         - intros [y Hcontr]; inversion Hcontr.
+         - intros Hsome.
+           destruct (decide (i = i0)). 
+           + subst.
+             rewrite insert_insert. 
+             unfold size, map_size.
+             do 2 (rewrite map_to_list_insert; auto).
+           + rewrite insert_commute;auto. 
+             unfold size, map_size.
+             rewrite map_to_list_insert;[|rewrite lookup_insert_ne;auto].
+             rewrite (map_to_list_insert _ i0);auto.
+             simpl. f_equal. apply IHm.
+             rewrite lookup_insert_ne in Hsome;auto. 
+  Qed.
+
+  Lemma revoke_list_related_sts_priv_cons W l i :
+    (is_Some (W.1.2 !! i) → W.1.2 !! i = Some (convert_rel (Rpub : relation region_type),
+                                               convert_rel (Rpriv : relation region_type))) →
+    related_sts_priv_world W (revoke_list l W) → related_sts_priv_world W (revoke_list (i :: l) W).
+  Proof.
+    intros Hstd Hpriv.
+    rewrite /revoke_list /=.
+    destruct (std_sta W !! i) eqn:Hsome; auto.
+    destruct (countable.encode Temporary =? p)%positive eqn:Htemp; auto.
+    destruct W as [ [Wstd_sta Wstd_rel] Wloc]. 
+    destruct Hpriv as [(Hdoms & Hdomr & Ha) Hloc]; auto.
+    split;simpl;auto.
+    rewrite /related_sts_priv.
+    apply Positive_as_OT.eqb_eq in Htemp. 
+    simpl in *. 
+    split;[|split].
+    - etrans;[|apply dom_insert_subseteq];auto.
+    - auto.
+    - intros j r1 r2 r1' r2' Hr Hr'.
+      rewrite Hr in Hr'. inversion Hr'. repeat (split;auto).
+      intros x y Hx Hy. 
+      destruct (decide (i = j)).
+      { subst. assert (is_Some (Wstd_rel !! j)) as Hasome; eauto.
+        rewrite Hstd in Hr; eauto. inversion Hr. 
+        rewrite Hsome in Hx. inversion Hx.
+        rewrite lookup_insert in Hy. inversion Hy.
+        right with (countable.encode Revoked);[|left].
+        right. cbv. exists Temporary, Revoked. 
+        split;[auto|split;[auto|] ].
+          by left. 
+      }
+      rewrite lookup_insert_ne in Hy;auto.
+      specialize (Ha j r1 r2 r1 r2 Hr Hr) as (_ & _ & Ha). 
+      subst. apply Ha; auto.
+  Qed. 
+
+  Lemma revoke_list_related_sts_priv W l :
+    (∀ (i : positive), is_Some(W.1.2 !! i) → W.1.2 !! i = Some (convert_rel (Rpub : relation region_type),
+                                                                convert_rel (Rpriv : relation region_type))) →
+    related_sts_priv_world W (revoke_list l W).
+  Proof.
+    induction l.
+    - split; apply related_sts_priv_refl.
+    - split;[|apply related_sts_priv_refl].
+      apply revoke_list_related_sts_priv_cons; auto. 
+  Qed.
+
+  Lemma revoke_related_sts_priv W :
+    (∀ (i : positive), is_Some(W.1.2 !! i) → W.1.2 !! i = Some (convert_rel (Rpub : relation region_type),
+                                                                convert_rel (Rpriv : relation region_type))) →
+    related_sts_priv_world W (revoke W).
+  Proof.
+    intros Hstd.
+    rewrite revoke_list_dom. apply revoke_list_related_sts_priv.
+    done. 
+  Qed.
+
+  Lemma revoke_list_size W l :
+    size (revoke_list l W).1.1 = size W.1.1. 
+  Proof.
+    induction l.
+    - done.
+    - destruct W as [Wstd Wloc].
+      destruct Wstd as [Wstd_sta Wstd_rel].
+      rewrite /= /std_sta /=. rewrite /= /std_sta /= in IHl. 
+      destruct (Wstd_sta !! a) eqn:Hsome.
+      + destruct (countable.encode Temporary =? p)%positive; auto.
+        rewrite (map_size_insert_Some); auto.
+        apply revoke_list_lookup_Some. eauto.
+      + apply IHl.
+  Qed.
+    
+  (* TODO: choose between:
+     1) restate revoke so that it only actually revokes the temporary in the M map
+     2) change region definition to related the domains of M and Wstd_sta to be equal
+        (we can argue that we want Wstd_sta to exactly represent the map M, and thus 
+        revoke should cover all temps in Wstd_sta)
+   *)
+
+  Lemma dom_equal_empty_inv_r Wstd_sta :
+    dom_equal Wstd_sta ∅ → Wstd_sta = ∅.
+  Proof.
+    intros Hdom. 
+    apply map_empty.
+    intros i.
+    destruct Hdom with i as [Hdom1 Hdom2]. 
+    apply eq_None_not_Some.
+    intros Hsome. specialize (Hdom1 Hsome) as [a [_ [x Hcontr] ] ].
+    inversion Hcontr.
+  Qed.
+
+  Lemma dom_equal_empty_inv_l M :
+    dom_equal ∅ M → M = ∅.
+  Proof.
+    intros Hdom. 
+    apply map_empty.
+    intros i.
+    destruct Hdom with (countable.encode i) as [Hdom1 Hdom2]. 
+    apply eq_None_not_Some.
+    intros Hsome.
+    assert (∃ a : Addr, countable.encode a = countable.encode i ∧ is_Some (M !! a)) as Ha; eauto.
+    specialize (Hdom2 Ha) as [x Hcontr].
+    inversion Hcontr.
+  Qed.
+
+  (* Lemma dom_equal_revoke W M : *)
+  (*   dom_equal (std_sta W) M → dom_equal (std_sta (revoke W)) M. *)
+  (* Proof. *)
+  (* Admitted. *)
   
+  (* Lemma dom_equal_insert_delete m M (x : positive) (a : Addr) : *)
+  (*   dom_equal (<[countable.encode a:=x]> m) M → *)
+  (*   dom_equal m (delete a M). *)
+  (* Proof. *)
+  (*   Admitted.  *)
+
+  Lemma related_sts_priv_weaken fs fr gs gr i x :
+    i ∉ dom (gset positive) fs →
+    related_sts_priv fs (<[i:=x]> gs) fr gr →
+    related_sts_priv fs gs fr gr.
+  Proof.
+    intros Hnin [Hdom_std [Hdom_loc Hrelated] ].
+    split;[|split;auto].
+    - rewrite dom_insert_L in Hdom_std.
+      apply elem_of_subseteq.
+      apply elem_of_subseteq in Hdom_std.
+      intros x' Hx'. specialize (Hdom_std x' Hx').
+      destruct (decide (x' = i)); [subst;contradiction|].
+      apply elem_of_union in Hdom_std as [Hcontr | Hgs]; auto.
+      apply elem_of_singleton_1 in Hcontr. contradiction. 
+    - intros i' r1 r2 r1' r2' Hr Hr'.
+      edestruct Hrelated as (Heq & Heq' & Hstate); eauto; subst.
+      repeat (split;auto).
+      intros x' y Hx' Hy.
+      destruct (decide (i = i')); subst.
+      + exfalso. apply Hnin. apply elem_of_gmap_dom. 
+        eauto.
+      + apply Hstate; auto.
+        rewrite lookup_insert_ne;auto. 
+  Qed.
+
+  Lemma big_sepM_exists {A B C : Type} `{EqDecision A, Countable A} (m : gmap A B) (φ : A → C -> B → iProp Σ) :
+    (([∗ map] a↦b ∈ m, ∃ c, φ a c b) ∗-∗ (∃ (m' : gmap A C), [∗ map] a↦c;b ∈ m';m, φ a c b))%I.
+  Proof.
+    iSplit. 
+    - iIntros "Hmap".
+      iInduction (m) as [| a x m Hnone] "IH" using map_ind.
+      + iExists empty. done.
+      + iDestruct (big_sepM_insert with "Hmap") as "[Hc Hmap]"; auto.
+        iDestruct "Hc" as (c) "Hc".
+        iDestruct ("IH" with "Hmap") as (m') "Hmap".
+        iExists (<[a:=c]> m').
+        iApply (big_sepM2_insert_2 with "Hc").
+        iFrame.
+    - iIntros "Hmap".
+      iDestruct "Hmap" as (m') "Hmap". 
+      iInduction (m) as [| a x m Hnone] "IH" using map_ind forall (m').
+      + done.
+      + iDestruct (big_sepM2_dom with "Hmap") as %Hdom. 
+        assert (is_Some (m' !! a)) as [ρ Hρ].
+        { apply elem_of_gmap_dom. rewrite Hdom dom_insert_L.
+          apply elem_of_union_l, elem_of_singleton; auto. }    
+        rewrite -(insert_id m' a ρ); auto.
+        rewrite -insert_delete. 
+        iDestruct (big_sepM2_insert with "Hmap") as "[Hφ Hmap]";[apply lookup_delete|auto|].
+        iApply big_sepM_insert;auto.
+        iDestruct ("IH" with "Hmap") as "Hmap". iFrame.
+        iExists ρ. iFrame. 
+  Qed. 
+  
+  Lemma monotone_revoke_list_region_def M W W' :
+    ⌜related_sts_priv_world W W'⌝ -∗
+     ⌜dom_equal (std_sta W') M⌝ -∗
+     sts_full_world sts_std (revoke W) -∗
+     region_map_def M (revoke W) -∗ region_map_def M (revoke W') (* ∗ sts_full_world sts_std (revoke W) *).
+  Proof.
+    iIntros (Hrelated Hdom) "Hfull Hr".
+    iDestruct (big_sepM_exists with "Hr") as (m') "Hr".
+    iDestruct (big_sepM2_sep with "Hr") as "[Hstates Hr]".
+    iAssert (∀ a ρ, ⌜m' !! a = Some ρ⌝ → ⌜ρ ≠ Temporary⌝)%I as %Htemp.
+    { iIntros (a ρ Hsome).
+      iDestruct (big_sepM2_lookup_1 _ _ _ a with "Hstates") as (γp) "[_ Hstate]"; eauto.
+      iDestruct (sts_full_state_std with "Hfull Hstate") as %Hρ.
+      iPureIntro. admit. 
+    }
+    iApply big_sepM_exists. iExists m'.
+    iApply big_sepM2_sep. iFrame. 
+    iApply (big_sepM2_mono with "Hr").
+    iIntros (a ρ γp Hsomeρ Hsomeγp) "Ha /=".
+    iDestruct "Ha" as (ρ) "(Hstate & Ha)".
+    
+
+    iDestruct (big_sepM2_sep with "[$Hstates $Hr]") as "Hr".
+    iDestruct (big_sepM_exists with "[Hr]") as "Hr".
+    { iExists m'. iFrame. }
+    iApply (big_sepM_mono with "Hr"). 
+    iIntros (a γp Hsome) "Ha /=".
+    iDestruct "Ha" as (ρ) "(Hstate & Ha)".
+    
+    
+  Lemma sts_full_world_std W W' :
+    (⌜related_sts_priv_world W W'⌝
+      -∗ sts_full_world sts_std W'
+    → ⌜∀ (i : positive), is_Some(W.1.2 !! i) → W.1.2 !! i = Some (convert_rel (Rpub : relation region_type),
+                                                                convert_rel (Rpriv : relation region_type))⌝)%I. 
+  Proof.
+    iIntros (Hrelated) "Hfull".
+    iDestruct "Hfull" as "[[% [% _] ] _]".
+    iPureIntro.
+    intros i Hx.
+    destruct Hrelated as [ (Hdom_std & Hdom_rel & Htransition) _].
+    assert ((∀ x : positive, x ∈ (dom (gset positive) W.1.2) → x ∈ (dom (gset positive) W'.1.2))) as H_std_elem_rel;
+      [by apply elem_of_subseteq|].
+    assert (i ∈ dom (gset positive) W.1.2) as H_i_rel; [by apply elem_of_dom|].
+    specialize (H_std_elem_rel i H_i_rel).
+    apply elem_of_dom in H_std_elem_rel as [ [r1' r2'] Hr'].
+    apply elem_of_dom in H_i_rel as [ [r1 r2] Hr].
+    specialize (Htransition i r1 r2 r1' r2' Hr Hr') as (Heq1 & Heq2 & _).
+    assert (is_Some (W'.1.2 !! i)) as Hsome'; eauto.    
+    rewrite H4 in Hr'; auto.
+    by inversion Hr'; subst. 
+  Qed.
+
+  Lemma monotone_revoke_list_sts_full_world M W l :
+    ⌜∀ (i : positive), i ∈ l→∃ (a : Addr), countable.encode a = i ∧ is_Some (M !! a)⌝ -∗
+    ⌜NoDup l⌝ -∗
+    sts_full_world sts_std W ∗ region_map_def M W
+    ==∗ (sts_full_world sts_std (revoke_list l W)
+          ∗ region_map_def M W).
+  Proof.
+    destruct W as [ [Wstd_sta Wstd_rel] Wloc]. 
+    rewrite /std_sta /=. 
+    iIntros (Hin Hdup) "[Hfull Hr]".
+    iInduction (l) as [|x l] "IH". 
+    - iFrame. done. 
+    - apply NoDup_cons in Hdup as [Hnin Hdup]. 
+      iMod ("IH" with "[] [] Hfull Hr") as "[Hfull Hr]"; auto.
+      { iPureIntro. intros a Ha. apply Hin. apply elem_of_cons. by right. }
+      rewrite /revoke_list /= /std_sta /=. 
+      destruct (Wstd_sta !! x) eqn:Hsome;[|by iFrame]. 
+      destruct (countable.encode Temporary =? p)%positive eqn:Htemp;[|by iFrame]. 
+      destruct Hin with x as [a [Heq [γp Hsomea] ] ];[apply elem_of_list_here|].
+      iDestruct (big_sepM_delete _ _ a with "Hr") as "[Hρ Hr]"; eauto.
+      iDestruct "Hρ" as (ρ') "(Hstate & Ha)".
+      iDestruct (sts_full_state_std with "Hfull Hstate") as %Hlookup. 
+      simpl in Hlookup. subst. rewrite revoke_list_not_elem_of_lookup in Hlookup; auto.
+      apply base.positive_beq_true in Htemp. 
+      rewrite Hsome -Htemp in Hlookup. inversion Hlookup; simplify_eq.
+      iMod (sts_update_std _ _ _ (Revoked) with "Hfull Hstate") as "[Hfull Hstate]".
+      iFrame.
+      iDestruct (big_sepM_delete _ _ a with "[$Hr Hstate]") as "$"; eauto.
+      iExists Revoked. iFrame.
+  Qed.
+
+  Lemma monotone_revoke_sts_full_world W :
+    sts_full_world sts_std W ∗ region W
+    ==∗ (sts_full_world sts_std (revoke W)
+          ∗ region W).
+  Proof.
+    iIntros "[Hfull Hr]".
+    rewrite region_eq /region_def.
+    iDestruct "Hr" as (M) "(HM & #Hdom & Hr)".
+    iDestruct "Hdom" as %Hdom. 
+    rewrite revoke_list_dom.
+    iMod (monotone_revoke_list_sts_full_world _ _ (map_to_list W.1.1).*1
+            with "[] [] [$Hfull $Hr]") as "[Hfull Hr]".
+    { iPureIntro. intros i Hin. apply map_to_list_fst in Hin as [x Hin].
+      destruct Hdom with i as [Hdom1 _].
+      apply Hdom1. exists x. by apply elem_of_map_to_list. 
+    }
+    { iPureIntro. apply NoDup_fst_map_to_list. }
+    iFrame.
+    iModIntro. iExists M. iFrame. done. 
+  Qed.
+
+  
+  
+  Lemma monotone_revoke W :
+    sts_full_world sts_std W ∗ region W ==∗ sts_full_world sts_std (revoke W) ∗ region (revoke W).
+  Proof.
+    iIntros "[HW Hr]".
+    iMod (monotone_revoke_sts_full_world with "[] [$HW Hr]") as "[HW Hr]".
+    rewrite region_eq /region_def.
+    iDestruct "Hr" as (M) "(HM & % & Hpreds)".
+    iDestruct (monotone_revoke_region_def with "Hpreds") as "Hpreds".
+    iModIntro. iFrame. iExists _. iFrame.
+    iPureIntro. by apply dom_equal_revoke.
+  Qed.     
+    
   Fixpoint delete_list {K V : Type} `{Countable K, EqDecision K}
              (ks : list K) (m : gmap K V) : gmap K V :=
     match ks with
@@ -237,12 +1326,24 @@ Section heap.
 
   Definition open_region_many_def (l : list Addr) (W : WORLD) : iProp Σ :=
     (∃ M, RELS M ∗
-         [∗ map] l↦γ ∈ (delete_list l M), ∃ γpred v p φ, ⌜γ = to_agree (γpred,p)⌝
-                                  ∗ ⌜p ≠ O⌝                                          
-                                  ∗ l ↦ₐ[p] v
-                                  ∗ future_mono φ
-                                  ∗ saved_pred_own γpred φ
-                                  ∗ ▷ φ (W,v))%I.
+         [∗ map] l↦γ ∈ (delete_list l M), ∃ ρ, sts_state_std (countable.encode l) ρ ∗
+                            match ρ with
+                            | Temporary => ∃ γpred (v : Word) (p : Perm) φ,
+                                               ⌜γ = to_agree (γpred,p)⌝
+                                             ∗ ⌜p ≠ O⌝
+                                             ∗ l ↦ₐ[p] v
+                                             ∗ future_pub_mono φ
+                                             ∗ saved_pred_own γpred φ
+                                             ∗ ▷ φ (W,v)
+                            | Permanent => ∃ γpred (v : Word) (p : Perm) φ,
+                                               ⌜γ = to_agree (γpred,p)⌝
+                                             ∗ ⌜p ≠ O⌝
+                                             ∗ l ↦ₐ[p] v
+                                             ∗ future_priv_mono φ
+                                             ∗ saved_pred_own γpred φ
+                                             ∗ ▷ φ (W,v)
+                            | Revoked => emp
+                            end)%I. 
   Definition open_region_many_aux : { x | x = @open_region_many_def }. by eexists. Qed.
   Definition open_region_many := proj1_sig open_region_many_aux.
   Definition open_region_many_eq : @open_region_many = @open_region_many_def := proj2_sig open_region_many_aux.
@@ -255,13 +1356,27 @@ Section heap.
     iFrame. 
   Qed.
 
-  Lemma region_open_next W φ ls l p :
-    l ∉ ls →
-    open_region_many ls W ∗ rel l p φ -∗
-    ∃ v, open_region_many (l :: ls) W ∗ l ↦ₐ[p] v ∗ ⌜p ≠ O⌝ ∗ ▷ future_mono φ ∗ ▷ φ (W,v). 
+  Lemma region_open_nil W :
+    (region W ∗-∗ open_region_many [] W)%I.
+  Proof.
+    iSplit; iIntros "H";
+    rewrite region_eq open_region_many_eq /=;
+            iFrame.
+  Qed.
+
+  Lemma region_open_next_temp W φ ls l p :
+    l ∉ ls → (std_sta W) !! (countable.encode l) = Some (countable.encode Temporary) -> 
+    open_region_many ls W ∗ rel l p φ ∗ sts_full_world W -∗
+                     ∃ v, sts_full_world W
+                        ∗ sts_state_std (countable.encode l) Temporary
+                        ∗ open_region_many (l :: ls) W
+                        ∗ l ↦ₐ[p] v
+                        ∗ ⌜p ≠ O⌝
+                        ∗ ▷ future_pub_mono φ
+                        ∗ ▷ φ (W,v). 
   Proof.
     rewrite open_region_many_eq . 
-    iIntros (Hnin) "[Hopen #Hrel]".
+    iIntros (Hnin Htemp) "(Hopen & #Hrel & Hfull)".
     rewrite /open_region_many_def /=. 
     rewrite rel_eq /rel_def /rel_def /region_def REL_eq RELS_eq /rel /region /REL /RELS. 
     iDestruct "Hrel" as (γpred) "#[Hγpred Hφ]".
@@ -271,15 +1386,20 @@ Section heap.
     rewrite delete_list_delete; auto. 
     rewrite HMeq big_sepM_insert; [|by rewrite lookup_delete]. 
     iDestruct "Hpreds" as "[Hl Hpreds]".
+    iDestruct "Hl" as (ρ) "[Hstate Hl]". destruct ρ. 
+    2: { iDestruct (sts_full_state_std with "Hfull Hstate") as %Hcontr.
+         rewrite Htemp in Hcontr. inversion Hcontr. apply countable.encode_inj in H4. done. }
+    2: { iDestruct (sts_full_state_std with "Hfull Hstate") as %Hcontr.
+         rewrite Htemp in Hcontr. inversion Hcontr. apply countable.encode_inj in H4. done. }    
     iDestruct "Hl" as (γpred' v p' φ') "(% & % & Hl & #Hmono & #Hφ' & Hφv)".  
-    inversion H2; subst.
+    inversion H3; subst.
     iDestruct (saved_pred_agree _ _ _ (W,v) with "Hφ Hφ'") as "#Hφeq".
     iExists _. iFrame.
     iSplitR "Hφv". 
     - rewrite /open_region.
       iExists _. repeat (rewrite -HMeq). iFrame "∗ #".
     - iSplitR;[auto|]. iSplitR.
-      + rewrite /future_mono.
+      + rewrite /future_pub_mono.
         iApply later_intuitionistically_2. iAlways.
         repeat (iApply later_forall_2; iIntros (?)).
         iDestruct (saved_pred_agree _ _ _ (a0,a1) with "Hφ Hφ'") as "#Hφeq'".
@@ -292,25 +1412,100 @@ Section heap.
         iRewrite "Hφeq". iFrame.
   Qed.
 
-  Lemma region_close_next W φ ls l p v :
+  Lemma region_open_next_perm W φ ls l p :
+    l ∉ ls → (std_sta W) !! (countable.encode l) = Some (countable.encode Permanent) -> 
+    open_region_many ls W ∗ rel l p φ ∗ sts_full_world W -∗
+                     ∃ v, sts_full_world W
+                        ∗ sts_state_std (countable.encode l) Permanent
+                        ∗ open_region_many (l :: ls) W
+                        ∗ l ↦ₐ[p] v
+                        ∗ ⌜p ≠ O⌝
+                        ∗ ▷ future_priv_mono φ
+                        ∗ ▷ φ (W,v). 
+  Proof.
+    rewrite open_region_many_eq . 
+    iIntros (Hnin Htemp) "(Hopen & #Hrel & Hfull)".
+    rewrite /open_region_many_def /=. 
+    rewrite rel_eq /rel_def /rel_def /region_def REL_eq RELS_eq /rel /region /REL /RELS. 
+    iDestruct "Hrel" as (γpred) "#[Hγpred Hφ]".
+    iDestruct "Hopen" as (M) "(HM & Hpreds)". 
+    iDestruct (reg_in γrel M with "[$HM $Hγpred]") as %HMeq.
+    rewrite HMeq delete_list_insert; auto.
+    rewrite delete_list_delete; auto. 
+    rewrite HMeq big_sepM_insert; [|by rewrite lookup_delete]. 
+    iDestruct "Hpreds" as "[Hl Hpreds]".
+    iDestruct "Hl" as (ρ) "[Hstate Hl]". destruct ρ. 
+    1: { iDestruct (sts_full_state_std with "Hfull Hstate") as %Hcontr.
+         rewrite Htemp in Hcontr. inversion Hcontr. apply countable.encode_inj in H4. done. }
+    2: { iDestruct (sts_full_state_std with "Hfull Hstate") as %Hcontr.
+         rewrite Htemp in Hcontr. inversion Hcontr. apply countable.encode_inj in H4. done. }    
+    iDestruct "Hl" as (γpred' v p' φ') "(% & % & Hl & #Hmono & #Hφ' & Hφv)".  
+    inversion H3; subst.
+    iDestruct (saved_pred_agree _ _ _ (W,v) with "Hφ Hφ'") as "#Hφeq".
+    iExists _. iFrame.
+    iSplitR "Hφv". 
+    - rewrite /open_region.
+      iExists _. repeat (rewrite -HMeq). iFrame "∗ #".
+    - iSplitR;[auto|]. iSplitR.
+      + iApply later_intuitionistically_2. iAlways.
+        repeat (iApply later_forall_2; iIntros (?)).
+        iDestruct (saved_pred_agree _ _ _ (a0,a1) with "Hφ Hφ'") as "#Hφeq'".
+        iDestruct (saved_pred_agree _ _ _ (a,a1) with "Hφ Hφ'") as "#Hφeq''".
+        iNext. iIntros (Hrel) "Hφw".
+        iRewrite ("Hφeq'"). 
+        iApply "Hmono"; eauto.
+        iRewrite -("Hφeq''"). iFrame. 
+      + iNext. 
+        iRewrite "Hφeq". iFrame.
+  Qed.
+
+  Lemma region_close_next_temp W φ ls l p v :
     l ∉ ls ->
-    open_region_many (l::ls) W ∗ l ↦ₐ[p] v ∗ ⌜p ≠ O⌝ ∗ future_mono φ ∗ ▷ φ (W,v) ∗ rel l p φ -∗ open_region_many ls W.
+    sts_state_std (countable.encode l) Temporary ∗
+                  open_region_many (l::ls) W ∗ l ↦ₐ[p] v ∗ ⌜p ≠ O⌝ ∗ future_pub_mono φ ∗ ▷ φ (W,v) ∗ rel l p φ
+                  -∗ open_region_many ls W.
   Proof.
     rewrite open_region_many_eq /open_region_many_def. 
-    iIntros (Hnin) "(Hreg_open & Hl & % & #Hmono & Hφ & #Hrel)".
+    iIntros (Hnin) "(Hstate & Hreg_open & Hl & % & #Hmono & Hφ & #Hrel)".
     rewrite rel_eq /rel_def REL_eq RELS_eq /rel /region /RELS /REL.
     iDestruct "Hrel" as (γpred) "#[Hγpred Hφ_saved]".
     iDestruct "Hreg_open" as (M) "(HM & Hpreds)".
     iDestruct (big_sepM_insert _ (delete l (delete_list ls M)) l with "[-HM]") as "test";
       first by rewrite lookup_delete.
-    { iFrame. iExists _,_,_,_. iFrame "∗ #". (iSplitR;[eauto|]). done. }
+    { iFrame. iExists _; iFrame. iExists _,_,_,_. iFrame "∗ #". (iSplitR;[eauto|]). done. }
     iExists _.
     iDestruct (reg_in γrel M with "[$HM $Hγpred]") as %HMeq.
     rewrite -delete_list_delete; auto. rewrite -delete_list_insert; auto.
     rewrite -HMeq. 
     iFrame "# ∗".
   Qed.
-    
+
+  Lemma region_close_next_perm W φ ls l p v :
+    l ∉ ls ->
+    sts_state_std (countable.encode l) Permanent ∗
+                  open_region_many (l::ls) W ∗ l ↦ₐ[p] v ∗ ⌜p ≠ O⌝ ∗ future_priv_mono φ ∗ ▷ φ (W,v) ∗ rel l p φ
+                  -∗ open_region_many ls W.
+  Proof.
+    rewrite open_region_many_eq /open_region_many_def. 
+    iIntros (Hnin) "(Hstate & Hreg_open & Hl & % & #Hmono & Hφ & #Hrel)".
+    rewrite rel_eq /rel_def REL_eq RELS_eq /rel /region /RELS /REL.
+    iDestruct "Hrel" as (γpred) "#[Hγpred Hφ_saved]".
+    iDestruct "Hreg_open" as (M) "(HM & Hpreds)".
+    iDestruct (big_sepM_insert _ (delete l (delete_list ls M)) l with "[-HM]") as "test";
+      first by rewrite lookup_delete.
+    { iFrame. iExists _; iFrame. iExists _,_,_,_. iFrame "∗ #". (iSplitR;[eauto|]). done. }
+    iExists _.
+    iDestruct (reg_in γrel M with "[$HM $Hγpred]") as %HMeq.
+    rewrite -delete_list_delete; auto. rewrite -delete_list_insert; auto.
+    rewrite -HMeq. 
+    iFrame "# ∗".
+  Qed.
+
+  (* ------------------------------- REVOCATION ------------------------------- *)
+  (* We now need to define a way to revoke all temporary regions of a world.
+     We will define a singular revoke action, which revokes a particulat location
+     and returns the given resources, with the updated Word. However, we require  *)
+  
 End heap. 
 
 Ltac auto_equiv :=
